# Serie 7: Folgen und Reihen

## 1.

> $a = \lim \limits _{n \to \infty}a_n$

### a)

> $$(a _n) = \left(\frac{2n^2 - n}{n^2 + n - 1}\right)$$

$$
\lim \limits _{n \to \infty}
=
\left.  \frac{2n^2 - n}{n^2 + n - 1}
\quad
\middle| \quad \times \frac{1 \over n^2}{1 \over n^2}
\right.
$$

$$
\lim \limits _{n \to \infty}
=
{2 - {1 \over n} \over 0 + {1 \over n} - {1 \over n^2}}
$$

$$
a_n
=
{2 - 0 \over 0 + 0 - 0}
$$

$$
a_n
=
{2 \over 0} = \underline{\underline{0}}
$$

### b)

> $$(a _n) = \left({3^n - 3^{n - 1} \over 2 + 3^n}\right)$$

$$
\lim \limits _{n \to \infty}
=
\left.  {3^n - 3^{n - 1} \over 2 + 3^n} \quad
\middle | \quad \times {3^{-n} \over 3^{-n}}
\right.
$$

$$
\lim \limits _{n \to \infty}
=
{1 - {1 \over 3} \over {1 \over 6^n} + 0}
$$

$$
a_n
=
{{2 \over 3} \over 0 + 0} = \underline{\underline{0}}
$$

### c)

> $$(a _n) = \left({3n - 2(-1)^n \over n}\right)$$

$$
\lim \limits _{n \to \infty}
=
\left. {3n - 2(-1)^n \over n} \quad
\middle | \quad \times {{1 \over n} \over {1 \over n}}
\right.
$$

$$
\lim \limits _{n \to \infty}
=
{3 - {-2^n \over n} \over 1}
$$

>$$
>\lim \limits _{n \to \infty}
>=
>\left. {-2^n \over n} \quad
>\middle | \quad \times {-2^{-n} \over -2^{-n}}
>\right.
>$$

>$$
>\lim \limits _{n \to \infty}
>=
>{1 \over -2n^{-n}}
>=
>{1 \over {1 \over -2n^{n}}}
>=
>{1 \over 0}
>=
>\underline{0}
>$$

$$
a_n
=
{3 - 0 \over 1} = \underline{\underline{3}}
$$

### d)

> $$(a _n) = \left( {\sqrt{4n^2 + n + 2} - \sqrt{4n^2 + 1}} \right )$$

$$
\lim \limits _{n \to \infty}
=
\left. {\sqrt{4n^2 + n + 2} - \sqrt{4n^2 + 1}} \quad
\middle | \quad \times {{\sqrt{4n^2 + n + 2} + \sqrt{4n^2 + 1}} \over {\sqrt{4n^2 + n + 2} + \sqrt{4n^2 + 1}}}
\right.
$$

$$
\lim \limits _{n \to \infty}
=
\left. {4n^2 + n + 2 - 4n^2 + 1 \over \sqrt{4n^2 + n + 2} + \sqrt{4n^2 + 1}} \quad
\middle | \quad \text{Umformung}
\right.
$$

$$
\lim \limits _{n \to \infty}
=
\left. {n + 3 \over (4n^2 + n + 2)^{{1 \over 2}} + (4n^2 + 1)^{1 \over 2}} \quad
\middle | \quad
\right.
$$

### e)

> $$(a _n) = \left( \left(1 + {1 \over 7n}\right)^n \right )$$

$$
\lim \limits _{n \to \infty}
=
\left. \left(1 + {1 \over 7n}\right)^n \quad
\middle | ^{7 {1 \over 7}}
\right.
$$

$$
\lim \limits _{n \to \infty}
=
\left(1 + {1 \over 7n}\right)^{7n \times {1 \over 7}}
$$

$$
a_n
=
\underline{\underline{e \over 7}}
$$

## 2.

### a)

### b)

### c)

## 3.

### a)

### b)

#### b1)

#### b2)

## 4.

### a)

### b)

### c)
