# Serie 3: Differentialrechnung

## 1.

> f(x) = x<sup>3</sup>

- a) [0,1]

  Steigung = (f(0 + 1) - f(0)) / 1

  = 1<sup>3</sup> - 0<sup>3</sup>

  = ***1***

- b) [1,2]

  Steigung = (f(1 + 2) - f(1)) / 2

  = (3^3 - 1^3) / 2

  = 26 / 2 = ***13***

- c) [-2, -1.5]

  Steigung = (f(-2 - 1.5) - f(-2)) / -1.5

  = ((-3.5)^3 - (-2)^3) / -1.5

  = (-42.875 - -8) / -1.5

  = -35.875 / -1.5

  = ***23.25***

- d) [x, x + h] fÃ¼r x e R, h > 0 beliebig

  Steigung = (f(x + h) - f(x)) / h

  = ((x + h)^3 - x^3) / h

  = (x^3 + 3x^2h + 3xh^2 + h^3 - x^3) / h

  = (3x^2h + 3xh^2 + h^3) / h

  = (h * (3x^2 + 3xh + h^2)) / h

  = ***3x^2 + 3xh + h^2***

## 2.

> Stelle: x = 1

- a) f(x) = x^6 - x^2 + 3

  - f'(x) = 6x^5 - 2x

  - f'(1) = 6 * 1^5 - 2 * 1

    = 6 - 2 = ***4***

- b) f(x) = x^7 + x^6

  - f'(x) = 7x^6 + 6x^5

  - f'(1) = 7 * 1^6 + 6 * 1^5

    = 7 + 6 = ***13***

- c) f(x) = x^5 + x^3 + 1

  - f'(x) = 5x^4 + 3x^2

  - f'(1) = 5 * 1^4 + 3 * 1^2

    = 5 + 3 = ***8***

## 3.

  y = (5x^3 - 4x)(x^2 + 5x)

  y = 5x^5 + 25x^4 - 4x^3 - 20x^2

  ***y' = 25x^4 + 100x^3 - 12x^2 - 40x***

## 4.

  - a)

  - b)

## 5.

  - a)

  - b)

## 6.

  f(x) = 1/x = x^-1

  f'(x) = -x^-2 = ***-1/x^2***
