# Serie 3: Differentialrechnung

## 1.

> $f(x) = x^3$

- a) $[0,1]$

  $\text{Steigung} = {f(0 + 1) - f(0) \over 1}$

  $= 1^3 - 0^3$

  $= \underline{\underline{1}}$

- b) $[1,2]$

  $\text{Steigung} = {f(1 + 2) - f(1) \over 2}$

  $= {3^3 - 1^3 \over 2}$

  $= {26 \over 2} = \underline{\underline{13}}$

- c) $[-2, -1.5]$

  $\text{Steigung} = {f(-2 - 1.5) - f(-2) \over -1.5}$

  $= {-3.5^3 - -2^3 \over -1.5}$

  $= {-42.875 - -8 \over -1.5}$

  $= {-35.875 \over -1.5}$

  $= \underline{\underline{23.25}}$

- d) $[x, x + h] \text{ fÃ¼r } x \in \mathbb{R}, h > 0 \text{ beliebig}$

  $\text{Steigung} = {f(x + h) - f(x) \over h}$

  $= {(x + h)^3 - x^3 \over h}$

  $= {x^3 + 3x^2h + 3xh^2 + h^3 - x^3 \over h}$

  $= {3x^2h + 3xh^2 + h^3 \over h}$

  $= {h(3x^2 + 3xh + h^2) \over h}$

  $= \underline{\underline{3x^2 + 3xh + h^2}}$

## 2.

> Stelle: $x = 1$

- a) $f(x) = x^6 - x^2 + 3$

  $f'(x) = 6x^5 - 2x$

  $f'(1) = 6 \times 1^5 - 2 \times 1$

  $= 6 - 2 = \underline{\underline{4}}$

- b) $f(x) = x^7 + x^6$

  $f'(x) = 7x^6 + 6x^5$

  $f'(1) = 7 \times 1^6 + 6 \times 1^5$

  $= 7 + 6 = \underline{\underline{13}}$

- c) $f(x) = x^5 + x^3 + 1$

  $f'(x) = 5x^4 + 3x^2$

  $f'(1) = 5 \times 1^4 + 3 \times 1^2$

  $= 5 + 3 = \underline{\underline{8}}$

## 3.

  $y = (5x^3 - 4x)(x^2 + 5x)$

  $y = 5x^5 + 25x^4 - 4x^3 - 20x^2$

  $\underline{\underline{y' = 25x^4 + 100x^3 - 12x^2 - 40x}}$

## 4.

  - a)

  - b)

## 5.

  - a)

  - b)

## 6.

  $f(x) = {1 \over x} = x^{-1}$

  $f'(x) = -x^{-2} = \underline{\underline{-{1 \over x^2}}}$
