# Serie 4: Integralrechnung

1.

  - a)

$$
\begin{align*}
  f(x) &= 2x^5 - 4x^3 + 6x^2 - 2 \\
  f'(x) &= 1/3 * x^6 - x^4 + 2x^3 - 2x + C
\end{align*}
$$

  - b) g(x) = -10x^4 + 2x^3 - 2

    ***G(x) = -2x^5 + 1/2 * x^4 - 2x + C***

  - c) h(x) = x^2 + 1/x^2 = x^2 + x^-2

    ***H(x) =*** 1/3 * x^3 - x^-1 + C = ***1/3 * x^3 - 1/x + C***

2.

  - a) f(x) = 1/2 * x^2 - 3x + C

    F(2) = 1/2 * 2^2 - 3*2 + C = 2 - 6 + C = C - 4

    => ***C =*** C = 9 + 4 = ***13***

  - b) f(x) = 1/3 * x^3 + x + C

    ***C = 8***

3.

  - a) I(3x^2 - 4x + 7)dx

    ***F(x) = x^3 - 2x^2 + 7x***

  - b) I(x + (x^2)/2)dx

    ***F(x) = (x^2)/2 + (x^3)/6***

  - c) I(9x^2 + 12x + 4)dx

    ***F(x) = 3x^3 + 6x^2 + 4x***

4.

  - a) I[1,2] (2x^3 + x^2 - 4x + 7)dx

    F(x) = (x^4)/2 + (x^3)/3 - 2x^2 + 7x + C

    F(1) = 1/2 + 1/3 - 2 + 7 = 35/6 + C

    F(2) = 8 + 8/3 - 8 + 14 = 50/3 + C

    ***F(2) - F(1) =*** 100/6 - 35/6 = ***65/6 + C***

  - b) I[-1,1] (4x^7 - 3x^3 + 6x^2 - 3)dx

    F(x) = (x^8)/2 - 3(x^4)/4 + 2x^3 - 3x + C

    F(-1) = 1/2 - 3/4 - 2 + 3 = 3/4 + C

    F(1) = 1/2 - 3/4 + 2 - 3 = -5/4 + C

    ***F(1) - F(-1) =*** -5/4 - 3/4 = ***-2 + C***

5.

  - a) I[0,4]  3(x^2)/4 dx

    F(x) = (x^3)/4 + C

    F(0) = 0 + C

    F(4) = (4^3)/4 = 16 + C

    ***F(4) - F(0) = 16 + C***

  - b) I[2,5]  x^2 dx

    F(x) = (x^3)/3 + C

    F(5) = (5^3)/3 = 125/3 + C

    F(2) = (2^3)/3 = 8/3 + C

    ***F(5) - F(2) =*** 125/3 - 8/3 = 117/3 = ***39 + C***

  - c) I[1,2]  4(x^3)/3 dx

    F(x) = (x^4)/3 + C

    F(2) = (2^4)/3 = 16/3 + C

    F(1) = (1^4)/3 = 1/3 + C

    ***F(2) - F(1) = 15/3 + C***

  - d) I[0,2]  (x^3 + 2x + 1) dx

    F(x) = (x^4)/4 + x^2 + x + C

    F(2) = (2^4)/4 + 2^2 + 2 = 16 + 4 + 2 = 22 + C

    F(0) = 0 + C

    ***F(2) - F(0) = 22 + C***

  - e) I[-3,4] 3(x^2)/7 dx

    F(x) = (x^3)/7 + C

    F(4) = (4^3)/7 = 64/7 + C

    F(-3) = (-3^3)/7 = -27/7 + C

    ***F(4) - F(3) =*** 64/7 - -27/7 = 91/7 = ***13 + C***

  - f) I[-1,3] (6x^2 - 4x - 6) dx

    F(x) = 2x^3 - 2x^2 - 6x + C

    F(3) = 2 * 3^3 - 2 * 3^2 - 6 * 3 = 54 - 18 - 18 = 18 + C

    F(-1) = 2(-1)^3 - 2(-1)^2 - 6(-1) = -2 - 1 - -6 = 3 + C

    ***F(3) - F(-1) =*** 18 - 3 = ***15 + C***

6.

  - a) f(x) = -x^2 + 3x - 2

    a = -1, b = 3, c = -2

    Nullstellen:

    x1 = (-3 + sqrt( (-3)^2 - 4*-1*-2 )) / 2*-1 = 1

    x2 = (-3 - sqrt( (-3)^2 - 4*-1*-2 )) / 2*-1 = 2

    F(x) = -(x^3)/3 + x^2 - 2x + C

    F(2) = -2/3 + C

    F(1) = -4/3 + C

    ***F(2) - F(1) =*** -2/3 - -4/3 + C = ***2/3 + C***

  - b)
