# Serie 7: Folgen und Reihen

## 1.

> $a = \lim \limits _{n \to \infty}a_n$

### a)

> $$(a _n) = \left(\frac{2n^2 - n}{n^2 + n - 1}\right)$$

$$
\begin{align*}
  \lim \limits _{n \to \infty} &= \frac{2n^2 - n}{n^2 + n - 1} &&| \ \cdot \frac{1 \over n^2}{1 \over n^2} \\
  \lim \limits _{n \to \infty} &= {2 - {1 \over n} \over 0 + {1 \over n} - {1 \over n^2}} &&| \ \lim \\
  a_n &= {2 - 0 \over 0 + 0 - 0} \\
  a_n &= {2 \over 0} \\
  &= 0
\end{align*}
$$

### b)

> $$(a _n) = \left({3^n - 3^{n - 1} \over 2 + 3^n}\right)$$

$$
\begin{align*}
  \lim \limits _{n \to \infty} &= {3^n - 3^{n - 1} \over 2 + 3^n} &&| \ \cdot {3^{-n} \over 3^{-n}} \\
  \lim \limits _{n \to \infty} &= {1 - {1 \over 3} \over {1 \over 6^n} + 0} &&| \ \lim \\
  a_n &= {{2 \over 3} \over 0 + 0} = 0
\end{align*}
$$

### c)

> $$(a _n) = \left({3n - 2(-1)^n \over n}\right)$$

$$
\begin{align*}
  \lim \limits _{n \to \infty} &= {3n - 2(-1)^n \over n} &&| \ \cdot {{1 \over n} \over {1 \over n}} \\
  \lim \limits _{n \to \infty} &= {3 - {-2^n \over n} \over 1}
\end{align*}
$$

>$$
>\lim \limits _{n \to \infty}
>=
>\left. {-2^n \over n} \quad
>\middle | \quad \cdot {-2^{-n} \over -2^{-n}}
>\right.
>$$

>$$
>\lim \limits _{n \to \infty}
>=
>{1 \over -2n^{-n}}
>=
>{1 \over {1 \over -2n^{n}}
>=
>{1 \over 0}
>=
>0}
>$$

$$
a_n
=
{3 - 0 \over 1} = 3
$$

### d)

> $$(a _n) = \left( {\sqrt{4n^2 + n + 2} - \sqrt{4n^2 + 1}} \right)$$

$$
\begin{align*}
  \lim \limits _{n \to \infty} &= {\sqrt{4n^2 + n + 2} - \sqrt{4n^2 + 1}} &&| \ \cdot {{\sqrt{4n^2 + n + 2} + \sqrt{4n^2 + 1}} \over {\sqrt{4n^2 + n + 2} + \sqrt{4n^2 + 1}}} \\
  \lim \limits _{n \to \infty} &= {4n^2 + n + 2 - 4n^2 + 1 \over \sqrt{4n^2 + n + 2} + \sqrt{4n^2 + 1}} &&| \ \text{Umformung} \\
  \lim \limits _{n \to \infty} &= {n + 3 \over (4n^2 + n + 2)^{{1 \over 2}} + (4n^2 + 1)^{1 \over 2}}
\end{align*}
$$

### e)

> $$(a _n) = \left( \left(1 + {1 \over 7n}\right)^n \right)$$

$$
\begin{align*}
  \lim \limits _{n \to \infty} &= \left(1 + {1 \over 7n}\right)^n &&| \ ^{7 {1 \over 7}} \\
  \lim \limits _{n \to \infty} &= \left(1 + {1 \over 7n}\right)^{7n \cdot {1 \over 7}} \\
  a_n &= {e \over 7}
\end{align*}
$$

## 2.

### a)

### b)

### c)

## 3.

### a)

### b)

#### b1)

#### b2)

## 4.

### a)

### b)

### c)
