# Serie 8: Reelle Funktionen

## 1.

### a)

$$
\begin{align*}
  &\lim\limits_{x \to \infty} {9x - 5 \over 7x + 3} & &| \quad \cdot {{1 \over x} \over {1 \over x}} \\
  &= \lim\limits_{x \to \infty} {9 - {5 \over x} \over 7 + {3 \over x}} & &| \quad \lim \\
  &= {9 - {5 \over \infty} \over 7 + {3 \over \infty}} \\
  &= {9 \over 7}
\end{align*}
$$

### b)

$$
\begin{align*}
  &\lim\limits_{x \to 5} {x + 1 \over x - 1} &&| \ \cdot {{1 \over x} \over {1 \over x}} \\
  &= \lim\limits_{x \to 5} {1 + {1 \over x} \over 1 - {1 \over x}} &&| \ \lim \\
  &= {{6 \over 5} \over {4 \over 5}} \\
  &= {6 \over 5} \cdot {5 \over 4} = {80 \over 20} = {8 \over 2} = 4
\end{align*}
$$

### c)

$$
\begin{align*}
  &\lim\limits_{x \to -1} {x^5 + 1 \over x + 1} &&| \ \cdot {{1 \over x^5} \over {1 \over x^5}} \\
  &= \lim\limits_{x \to -1} {1 + {1 \over x^5} \over {1 \over x^4} + {1 \over x^5}} &&| \ \lim \\
  &= {1 - 1 \over 1 - 1} = {0 \over 0} = 1
\end{align*}
$$

### d)

$$
\begin{align*}
  &\lim\limits_{x \to 1} {x^2 - 1 \over x^2 + 1} &&| \ \cdot {{1 \over x^2} \over {1 \over x^2}} \\
  &= \lim\limits_{x \to 1} {1 - {1 \over x^2} \over 1 + {1 \over x^2}} &&| \ \lim \\
  &= {1 - {1 \over 1} \over 1 + {1 \over 1}} = {0 \over 2} = 0
\end{align*}
$$

### e)

$$
\begin{align*}
 &\lim\limits_{x \to - \infty} {x^2 - 5x + 3 \over 7x^2 + 1} &&| \ \cdot {{1 \over x^2} \over {1 \over x^2}} \\
 &= \lim\limits_{x \to - \infty} {1 - {5x \over x^2} + {3 \over x^2} \over 7 + {1 \over x^2}} \\
 &= \lim\limits_{x \to - \infty} -{5x \over x^2} &&| \ \cdot {{1 \over x} \over {1 \over x}} \\
 &= \lim\limits_{x \to - \infty} -{5 \over x} &&| \ \lim \\
 &= -{5 \over -\infty} = 0 \\
 &= \lim\limits_{x \to - \infty} {1 - 0 + {3 \over x^2} \over 7 + {1 \over x^2}} &&| \ \lim \\
 &= {1 + 0 \over 7 + 0} = {1 \over 7}
\end{align*}
$$

## 2.

### a)

$$
\begin{align*}
 &\lim\limits_{x\to 1} {3x-3 \over x^2+2x-3} &&| \ \cdot {{1 \over x} \over {1 \over x}} \\
 &= \lim\limits_{x\to 1} {3-{3 \over x} \over x+2-{3 \over x}} &&| \ \lim \\
 &= {3-{3 \over 1} \over 1+2-{3 \over 1}} = {0 \over 0} = 1
\end{align*}
$$

### b)

$$
\lim\limits_{x\to0} h(x), \text{ where } h(x) =
  \begin{cases}
    2x-3 & (x < 0)\\
    2x+5 & (x > 0)
  \end{cases}
$$

$$\lim\limits_{x\to0} 2x-3 \ | \ x < 0 = -3$$
$$\lim\limits_{x\to0} 2x+5 \ | \ x > 0 = 5$$

### c)

$$
\begin{align*}
  &\lim\limits_{x\to\infty} {30 \over 5 + 4e^{-2x}} \\
  &= \lim\limits_{x\to\infty} {30 \over 5 + {4 \over e^{2x}}} &&| \ \lim \\
  &= {30 \over 5 + {4 \over \infty}} = {30 \over 5} = 6
\end{align*}
$$

### d)

$$\lim\limits_{x\to\infty} \left(\left({5x^3-4x^4 \over x^2+8x^4+5x^3}\right)^3 \cdot -{5x-2 \over -2x+5}\right)$$

### e)

$$
\begin{align*}
  &\lim\limits_{x\to\infty} {1-x \over 1-\sqrt{x}} &&| \ \cdot {{1 \over x} \over {1 \over x}} \\
  &= \lim\limits_{x\to\infty} {{1 \over x}-1 \over {1 \over x}-{1 \over \sqrt{x}}} &&| \ \lim \\
  &= {0-1 \over 0-0} = {-1 \over 0}
\end{align*}
$$

## 3.

$$
\begin{align*}
  &\lim\limits_{x\to4} {x^2+x-20 \over x-4} &&| \ \cdot {{1 \over x} \over {1 \over x}} \\
  &= \lim\limits_{x\to4} {x+1-{20 \over x} \over 1-{4 \over x}} &&| \ \cdot {{1 \over x} \over {1 \over x}}
\end{align*}
$$

## 4.

## 5.

### a)

### b)

## 6.
